Take advantage of ARMv6T2/ARMv7 instructions even if not in Thumb2 mode  (#203)
* Clarify that ARMv6 is in fact ARMv6T2

The ARMv6 comes in two flavors depending on the version of the Thumb
instruction set supported: ARMv6 for the original Thumb, ARMv6T2 for Thumb2.
CompCert only supports Thumb2, so its ARMv6 architecture should really be
called ARMv6T2. This makes a difference: the GNU assembler rejects most of
the instructions CompCert generates for ARMv6 with "-mthumb" if the
architecture is specified as ".arch armv6" as opposed to ".arch armv6t2".

This patch fixes the architecture specification in the target printer and
the internal name of the architecture. It does not change the configure
script's flags to avoid breaking changes.

* Always use ARM movw/movt to load large immediates

These move-immediate instructions used to be only emitted in Thumb mode, not
in ARM mode. As far as I understand ARM's documentation, these instructions
are available in *both* modes in ARMv6T2 and above. This should cover all of
CompCert's ARM targets.

Tested for ARMv6 and ARMv7, both with and without Thumb2. The behavior is
now identical to Clang, and the GNU assembler accepts these instructions in
all configurations.

* Separate ARMv6 and ARMv6T2; no movw/movt on ARMv6

- define separate architecture models for ARMv6 and ARMv6T2
- introduce `Archi.move_imm` parameter on ARM to identify models with
  `movw`/`movt` move-immediate instructions (all except ARMv6, in both ARM
  and Thumb mode)

* Fixes for support for architectures with Thumb2

- rename relevant parameter to `Archi.thumb2_support`
- on ARMv6 without Thumb2, silently accept -marm flag (but not -mthumb)
- allow generation of `sbfx` in ARM mode if Thumb2 is supported

driver/Driver.ml
@@ -205,7 +205,8 @@ let version_string =
   else
     "The CompCert C verified compiler, version "^ Version.version ^ "\n"
 
-let target_help = if Configuration.arch = "arm" then
+let target_help =
+  if Configuration.arch = "arm" && Configuration.model <> "armv6" then
 {|Target processor options:
   -mthumb        Use Thumb2 instruction encoding
   -marm          Use classic ARM instruction encoding
@@ -372,8 +373,11 @@ let cmdline_actions =
   Exact "-conf", Ignore; (* Ignore option since it is already handled *)
   Exact "-target", Ignore;] @ (* Ignore option since it is already handled *)
   (if Configuration.arch = "arm" then
-    [ Exact "-mthumb", Set option_mthumb;
-      Exact "-marm", Unset option_mthumb; ]
+    if Configuration.model = "armv6" then
+      [ Exact "-marm", Ignore ] (* Thumb needs ARMv6T2 or ARMv7 *)
+    else
+      [ Exact "-mthumb", Set option_mthumb;
+        Exact "-marm", Unset option_mthumb; ]
   else []) @
 (* Assembling options *)
   assembler_actions @
