runtime/arm/sysdeps.h
@@ -86,6 +86,8 @@ f:
 	.syntax unified
 #if defined(MODEL_armv6)
         .arch   armv6
+#elif defined(MODEL_armv6t2)
+        .arch   armv6t2
 #elif defined(MODEL_armv7a)
         .arch   armv7-a
 #elif defined(MODEL_armv7r)
