arm/Asmgen.v
@@ -162,7 +162,7 @@ Definition iterate_op (op1 op2: shift_op -> instruction) (l: list int) (k: code)
 
 (** Smart constructors for integer immediate arguments. *)
 
-Definition loadimm_thumb (r: ireg) (n: int) (k: code) :=
+Definition loadimm_word (r: ireg) (n: int) (k: code) :=
   let hi := Int.shru n (Int.repr 16) in
   if Int.eq hi Int.zero
   then Pmovw r n :: k
@@ -177,8 +177,8 @@ Definition loadimm (r: ireg) (n: int) (k: code) :=
     Pmov r (SOimm n) :: k
   else if Nat.leb l2 1%nat then
     Pmvn r (SOimm (Int.not n)) :: k
-  else if thumb tt then
-    loadimm_thumb r n k
+  else if Archi.thumb2_support then
+    loadimm_word r n k
   else if Nat.leb l1 l2 then
     iterate_op (Pmov r) (Porr r r) d1 k
   else
@@ -365,14 +365,14 @@ Definition transl_op
       OK (addimm r IR13 (Ptrofs.to_int n) k)
   | Ocast8signed, a1 :: nil =>
       do r <- ireg_of res; do r1 <- ireg_of a1;
-      OK (if thumb tt then
+      OK (if Archi.thumb2_support then
             Psbfx r r1 Int.zero (Int.repr 8) :: k
           else
             Pmov r (SOlsl r1 (Int.repr 24)) ::
             Pmov r (SOasr r (Int.repr 24)) :: k)
   | Ocast16signed, a1 :: nil =>
       do r <- ireg_of res; do r1 <- ireg_of a1;
-      OK (if thumb tt then
+      OK (if Archi.thumb2_support then
             Psbfx r r1 Int.zero (Int.repr 16) :: k
           else
             Pmov r (SOlsl r1 (Int.repr 16)) ::
