arm/Archi.v
@@ -65,3 +65,7 @@ Global Opaque ptr64 big_endian splitlong
 
 Inductive abi_kind := Softfloat | Hardfloat.
 Parameter abi: abi_kind.
+
+(** Whether instructions added with Thumb2 are supported. True for ARMv6T2
+  and above. *)
+Parameter thumb2_support: bool.
